Implement an hollow model and extract the code from the hollow model

src/model/Isolation/IsolationTypes.v
@@ -1,57 +1,70 @@
 Require Import List Arith.
+Require Import Coq.Program.Tactics.
+
+From Pip.Model.Meta Require Import TypesModel.
+
+Module IsolationTypes <: TypesModel.
 
   (* Types *)
-  Axiom tableSize nbLevel nbPage maxVint contextSize : nat.
-  Axiom nbLevelNotZero: nbLevel > 0.
-  Axiom nbPageNotZero: nbPage > 0.
-  Axiom maxVintNotZero: maxVint > 0.
-  Axiom contextSizeNotZero: contextSize > 0.
-  Axiom contextSizeLessThanTableSize: contextSize < tableSize.
+  Parameter tableSize : nat.
+  Parameter nbPage : nat.
+  Parameter nbLevel : nat.
+  Parameter maxVint : nat.
 
-  Axiom tableSizeIsEven : Nat.Even tableSize.
-  (* END NOT SIMULATION *)
-  Definition tableSizeLowerBound := 14.
-  Axiom tableSizeBigEnough : tableSize > tableSizeLowerBound. (* to be fixed on count **) 
-  Record index := {
+  Record index_s := {
     i :> nat ;
     Hi : i < tableSize
   }.
 
-  Record page := { 
+  Definition index := index_s.
+
+  Record page_s := { 
     p :> nat;
     Hp : p < nbPage
   }.
 
+  Definition page := page_s.
+
   Definition paddr := (page * index)%type.
 
-  Record vaddr := {
+  Record vaddr_s := {
     va :> list index ;
     Hva : length va = nbLevel + 1
   }.
 
-  Record level := {
+  Definition vaddr := vaddr_s.
+
+  Record level_s := {
     l :> nat ;
     Hl : l < nbLevel
   }.
 
-  Record count := {
+  Definition level := level_s.
+
+  Record count_s := {
     c :> nat ;
     Hnb : c <= (3*nbLevel) + 1;
   }.
 
-  Record boolvaddr := {
+  Definition count := count_s.
+
+  Record boolvaddr_s := {
     success : bool;
     FFvaddr : vaddr;
   }.
+
+  Definition boolvaddr := boolvaddr_s.
 
   Definition userValue := nat.
   Definition vint := nat.
   Definition contextAddr := nat.
 
-  Record interruptMask := {
+  Record interruptMask_s := {
     m :> list bool;
     Hm : length m = maxVint+1;
   }.
+
+  Definition interruptMask := interruptMask_s.
 
   Parameter index_d : index.
   Parameter page_d : page.
@@ -59,57 +72,39 @@ Require Import List Arith.
   Parameter count_d : count.
   Parameter int_mask_d : interruptMask.
 
-  Require Import Coq.Program.Tactics.
-
   Program Definition CIndex  (p : nat) : index :=
     if (lt_dec p tableSize) then
-      Build_index p _ else index_d.
+      Build_index_s p _ else index_d.
 
   Program Definition CPage (p : nat) : page :=
     if (lt_dec p nbPage) then
-      Build_page p _ else page_d.
+      Build_page_s p _ else page_d.
 
   Program Definition CVaddr (l: list index) : vaddr := 
     if (Nat.eq_dec (length l) (nbLevel+1))
-      then Build_vaddr l _
+      then Build_vaddr_s l _
     else
-      Build_vaddr (repeat (CIndex 0) (nbLevel+1)) _.
-
-
-(* BEGIN NOT SIMULATION *)
+      Build_vaddr_s (repeat (CIndex 0) (nbLevel+1)) _.
 
   Next Obligation.
   apply repeat_length.
   Qed.
 
-(* END NOT SIMULATION *)
-
   Program Definition CLevel ( a :nat) : level := 
     if lt_dec a nbLevel then
-      Build_level a _
+      Build_level_s a _
     else level_d .
 
   Program Definition CCount ( a :nat) : count := 
     if le_dec a ((3*nbLevel) + 1) then
-      Build_count a _
+      Build_count_s a _
     else count_d .
 
   Program Definition CIntMask (m : list bool) : interruptMask :=
     if Nat.eq_dec (length m) (maxVint+1) then
-      Build_interruptMask m _
+      Build_interruptMask_s m _
     else int_mask_d.
 
-(* Inductive yield_checks : Type :=
-| FAIL_INVALID_INT_LEVEL_Cons
-| FAIL_INVALID_CTX_SAVE_INDEX_Cons
-| FAIL_CALLER_CONTEXT_SAVE_Cons
-| FAIL_UNAVAILABLE_TARGET_VIDT_Cons
-| FAIL_UNAVAILABLE_TARGET_CTX_Cons
-| FAIL_UNAVAILABLE_CALLER_VIDT_Cons
-| FAIL_ROOT_CALLER_Cons
-| FAIL_INVALID_CHILD_Cons
-| FAIL_MASKED_INTERRUPT_Cons
-| SUCCESS_Cons. *)
 Inductive yield_checks : Type :=
 | FAIL_INVALID_INT_LEVEL
 | FAIL_INVALID_CTX_SAVE_INDEX
@@ -121,3 +116,5 @@ Inductive yield_checks : Type :=
 | FAIL_INVALID_CHILD
 | FAIL_MASKED_INTERRUPT
 | SUCCESS.
+
+End IsolationTypes.
