src/model/Hollow/HollowModel.v
@@ -1,0 +1,85 @@
+From Pip.Model.Meta Require Import TypesModel StateModel InterfaceModel StateAgnosticMonad.
+Require Import Bool.
+
+Module HollowTypes <: TypesModel.
+
+  Parameter index : Type.
+  Parameter index_d : index.
+  Parameter page  : Type.
+  Parameter page_d : page.
+  Parameter paddr : Type.
+  Parameter vaddr : Type.
+  Parameter level : Type.
+  Parameter level_d : level.
+  Parameter count : Type.
+  Parameter count_d : count.
+  Parameter boolvaddr : Type.
+  Parameter userValue : Type.
+  Parameter contextAddr : Type.
+  Parameter interruptMask : Type.
+  Parameter int_mask_d : interruptMask.
+
+  Inductive yield_checks : Type :=
+| FAIL_INVALID_INT_LEVEL
+| FAIL_INVALID_CTX_SAVE_INDEX
+| FAIL_CALLER_CONTEXT_SAVE
+| FAIL_UNAVAILABLE_TARGET_VIDT
+| FAIL_UNAVAILABLE_TARGET_CTX
+| FAIL_UNAVAILABLE_CALLER_VIDT
+| FAIL_ROOT_CALLER
+| FAIL_INVALID_CHILD
+| FAIL_MASKED_INTERRUPT
+| SUCCESS.
+
+End HollowTypes.
+
+Module HollowState <: StateModel.
+
+  Parameter state : Type.
+
+End HollowState.
+
+Module HollowInterface <: (InterfaceModel HollowTypes HollowState).
+
+  Module SAMM := StateAgnosticMonad HollowState.
+  Export SAMM.
+  Import HollowTypes.
+
+  Parameter getCurPartition : SAM page.
+  Parameter updateCurPartition : page -> SAM unit.
+  Parameter readVirtual    : page -> index -> SAM vaddr.
+  Parameter readPhysical    : page -> index -> SAM page.
+  Parameter readVirEntry    : page -> index -> SAM vaddr.
+  Parameter readPhyEntry    : page -> index -> SAM page.
+  Parameter writeVirtual    : page -> index -> vaddr -> SAM unit.
+  Parameter writePhysical    : page -> index -> page -> SAM unit.
+  Parameter writeVirEntry    : page -> index -> vaddr -> SAM unit.
+  Parameter writePhyEntry    : page -> index -> page -> bool -> bool -> bool -> bool -> bool -> SAM unit.
+  Parameter mapKernel    : page -> index -> SAM unit.
+  Parameter readAccessible    : page -> index -> SAM bool.
+  Parameter writeAccessible    : page -> index -> bool -> SAM unit.
+  Parameter readPresent    : page -> index -> SAM bool.
+  Parameter writePresent    : page -> index -> bool -> SAM unit.
+  Parameter readPDflag    : page -> index -> SAM bool.
+  Parameter writePDflag    : page -> index -> bool -> SAM unit.
+  Parameter readIndex    : page -> index -> SAM index.
+  Parameter writeIndex    : page -> index -> index -> SAM unit.
+  Parameter getMaxIndex    : SAM index.
+  Parameter checkRights    : bool -> bool -> bool -> SAM bool.
+  Parameter maxFreeLL    : SAM index.
+  Parameter getIndexOfAddr    : vaddr -> level -> SAM index.
+  Parameter getNbLevel    : SAM level.
+  Parameter prepareType    : bool -> vaddr -> SAM boolvaddr.
+  Parameter getPd    : page -> SAM page.
+  Parameter readVirtualUser    : page -> index -> SAM vaddr.
+  Parameter fetchVirtual    : vaddr -> index -> SAM vaddr.
+  Parameter storeVirtual    : vaddr -> index -> vaddr -> SAM unit.
+  Parameter setInterruptMask    : interruptMask -> SAM unit.
+  Parameter getInterruptMaskFromCtx    : contextAddr -> SAM interruptMask.
+  Parameter noInterruptRequest : interruptMask -> SAM bool.
+  Parameter updateMMURoot    : page -> SAM unit.
+  Parameter getMultiplexer    : SAM page.
+  Parameter page_eqb    : page -> page -> SAM bool.
+  Parameter loadContext    : contextAddr -> bool -> SAM unit.
+
+End HollowInterface.
