src/model/Isolation/IsolationStateMonad.v
@@ -1,0 +1,443 @@
+From Pip.Model.Meta Require Import TypesModel StateModel StateAgnosticMonad InterfaceModel.
+From Pip.Model.Isolation Require Import IsolationTypes.
+
+Require Import Coq.Strings.String Lia NPeano.
+Require Import Arith Bool List.
+Import List.ListNotations.
+
+Module IsolationState <: StateModel.
+
+Export IsolationTypes.
+
+  Record Pentry : Type:=
+  {
+    read    : bool;
+    write   : bool;
+    exec    : bool;
+    present : bool;
+    user    : bool;
+    pa      : page
+  }.
+
+  Record Ventry : Type:=
+  {
+    pd : bool;
+    va : vaddr
+  }.
+
+  Inductive value : Type := 
+  |PE : Pentry -> value
+  |VE : Ventry -> value
+  |PP : page -> value
+  |VA : vaddr -> value
+  |I  : index -> value
+  |U  : userValue -> value.
+
+  Record IsolationState : Type := {
+    currentPartition : page;
+    memory : list (paddr * value)
+  }.
+
+  Definition state := IsolationState.
+
+End IsolationState.
+
+Module IsolationStateMonad <: InterfaceModel IsolationTypes IsolationState.
+
+  Module SAMM := StateAgnosticMonad IsolationState.
+  Export SAMM.
+
+  Fixpoint eqList {A : Type} (l1 l2 : list A) (eq : A -> A -> bool) : bool :=
+  match l1, l2 with
+  | nil, nil       => true
+  | a::l1', b::l2' => if eq a b then eqList l1' l2' eq else false
+  | _ , _          => false
+  end.
+
+  Definition beqIndex (a b : index) : bool := a =? b.
+  Definition beqPage (a b : page) : bool := a =? b.
+  Definition beqVAddr (a b : vaddr) : bool := eqList a b beqIndex.
+
+  Definition beqPairs {A B: Type} (a : (A * B)) (b : (A * B))
+                                  (eqA : A -> A -> bool) (eqB : B -> B -> bool) :=
+    if (eqA (fst a) (fst b)) && (eqB (snd a) (snd b)) then
+      true
+    else false.
+
+  Fixpoint lookup {A B C: Type} (k : A) (i : B) (assoc : list ((A * B) * C))
+                                (eqA : A -> A -> bool) (eqB : B -> B -> bool) :=
+  match assoc with
+  | nil => None
+  | (a, b) :: assoc' =>
+    if beqPairs a (k,i) eqA eqB then
+      Some b
+    else
+      lookup k i assoc' eqA eqB
+  end.
+
+  Definition getCurPartition : SAM page :=
+    perform s := get in ret (currentPartition s).
+
+  Definition updateCurPartition (p : page) : SAM unit :=
+    modify (fun s => {| currentPartition := p; memory := s.(memory) |}).
+
+  Definition readVirtual (p : page) (idx : index) : SAM vaddr :=
+  perform s := get in
+  let entry := lookup p idx (memory s) beqPage beqIndex in
+  match entry with
+  | Some (VA a) => ret a
+  | Some _      => undefined "Error : expected to find a virtual address, but found another type"
+  | None        => undefined "Error : no value at this address"
+  end.
+
+  Definition readPhysical (p : page) (idx : index) : SAM page :=
+  perform s := get in
+  let entry := lookup p idx (memory s) beqPage beqIndex in
+  match entry with
+  | Some (PP page) => ret page
+  | Some _      => undefined "Error : expected to find a physical page, but found another type"
+  | None        => undefined "Error : no value at this address"
+  end.
+
+  Definition readVirEntry (p : page) (idx : index) : SAM vaddr :=
+  perform s := get in
+  let entry := lookup p idx (memory s) beqPage beqIndex in
+  match entry with
+  | Some (VE vir_entry) => ret (va vir_entry)
+  | Some _      => undefined "Error : expected to find a virtual entry, but found another type"
+  | None        => undefined "Error : no value at this address"
+  end.
+
+  Definition readPhyEntry (p : page) (idx : index) : SAM page :=
+  perform s := get in
+  let entry := lookup p idx (memory s) beqPage beqIndex in
+  match entry with
+  | Some (PE phy_entry) => ret (pa phy_entry)
+  | Some _      => undefined "Error : expected to find a physical entry, but found another type"
+  | None        => undefined "Error : no value at this address"
+  end.
+
+  Fixpoint removeDup {A B C: Type} (k : A) (i : B) (assoc : list ((A * B) * C))
+                                   (eqA : A -> A -> bool) (eqB : B -> B -> bool) :=
+  match assoc with
+    | nil => nil
+    | (a, b) :: assoc' => if beqPairs a (k,i) eqA eqB then
+                            removeDup k i assoc' eqA eqB
+                          else (a, b) :: (removeDup k i assoc' eqA eqB)
+  end.
+
+  Definition add {A B C: Type} (k : A) (i : B) (v : C) (assoc : list ((A * B) * C))
+                               (eqA : A -> A -> bool) (eqB : B -> B -> bool) :=
+    (k, i, v) :: removeDup k i assoc eqA eqB.
+
+  Definition writeVirtual (paddr : page) (idx : index) (va : vaddr) : SAM unit :=
+  modify (fun s => {|
+    currentPartition := s.(currentPartition);
+    memory := add paddr idx (VA va) (memory s) beqPage beqIndex
+  |}).
+
+  Definition writePhysical (paddr : page) (idx : index) (p : page) : SAM unit :=
+  modify (fun s => {|
+    currentPartition := s.(currentPartition);
+    memory := add paddr idx (PP p) (memory s) beqPage beqIndex
+  |}).
+
+  Definition writeVirEntry (paddr : page) (idx : index) (va : vaddr) : SAM unit :=
+  let vir_entry := {| pd := false ; va := va |} in
+  modify (fun s => {|
+    currentPartition := s.(currentPartition);
+    memory := add paddr idx (VE vir_entry) (memory s) beqPage beqIndex
+  |}).
+
+  Definition writePhyEntry (paddr : page) (idx : index) (pa : page) (p u r w e : bool) :=
+  let phy_entry := {| read := r; write := w ; exec := e; present := p ; user := u ; pa := pa |} in
+  modify (fun s => {|
+    currentPartition := (currentPartition s) ;
+    memory := add paddr idx (PE phy_entry) (memory s) beqPage beqIndex
+  |}).
+
+  Definition defaultPage := CPage 0.
+
+  Definition mapKernel (paddr : page) (idx : index) :=
+  let kernel_entry := {| read := false;
+                         write := false;
+                         exec := false;
+                         present := false;
+                         user := false;
+                         pa := defaultPage
+                      |} in
+  modify (fun s =>
+  {|
+    currentPartition := (currentPartition s) ;
+    memory := add paddr idx (PE kernel_entry) (memory s) beqPage beqIndex
+  |}).
+
+  Definition readAccessible (p : page) (idx : index) : SAM bool :=
+  perform s := get in
+  let entry := lookup p idx (memory s) beqPage beqIndex in
+  match entry with
+  | Some (PE phy_entry) => ret (user phy_entry)
+  | Some _              => undefined "Error : expected to find a physical entry, but found another type"
+  | None                => undefined "Error : no value at this address"
+  end.
+
+  Definition writeAccessible (p : page) (idx : index) (flag : bool) : SAM unit:=
+  perform s := get in
+  let entry :=  lookup p idx (memory s) beqPage beqIndex in
+  match entry with
+  | Some (PE phy_entry) =>
+    let newEntry :=
+      {|
+        read    := (read    phy_entry);
+        write   := (write   phy_entry);
+        exec    := (exec    phy_entry);
+        present := (present phy_entry);
+        user    := flag;
+        pa      := (pa      phy_entry)
+      |} in
+    modify (fun s =>
+      {|
+        currentPartition := (currentPartition s);
+        memory := add p idx (PE newEntry) (memory s) beqPage beqIndex
+      |})
+  | Some _ => undefined "Error : expected to find a physical entry, but found another type"
+  | None   => undefined "Error : no value at this address"
+  end.
+
+  Definition readPresent (p : page) (idx : index) : SAM bool :=
+  perform s := get in
+  let entry := lookup p idx (memory s) beqPage beqIndex in
+  match entry with
+  | Some (PE phy_entry) => ret (present phy_entry)
+  | Some _              => undefined "Error : expected to find a physical entry, but found another type"
+  | None                => undefined "Error : no value at this address"
+  end.
+
+  Definition writePresent (p : page) (idx : index) (flag : bool) : SAM unit:=
+  perform s := get in
+  let entry :=  lookup p idx (memory s) beqPage beqIndex in
+  match entry with
+  | Some (PE phy_entry) =>
+    let newEntry :=
+      {|
+        read    := (read  phy_entry);
+        write   := (write phy_entry);
+        exec    := (exec  phy_entry);
+        present := flag             ;
+        user    := (user  phy_entry);
+        pa      := (pa    phy_entry)
+      |} in
+    modify (fun s =>
+      {|
+        currentPartition := (currentPartition s);
+        memory := add p idx (PE newEntry) (memory s) beqPage beqIndex
+      |})
+  | Some _ => undefined "Error : expected to find a physical entry, but found another type"
+  | None   => undefined "Error : no value at this address"
+  end.
+
+  Definition readPDflag (p : page) (idx : index) : SAM bool :=
+  perform s := get in
+  let entry :=  lookup p idx (memory s) beqPage beqIndex in
+  match entry with
+  | Some (VE vir_entry) => ret (pd vir_entry)
+  | Some _              => undefined "Error : expected to find a virtual entry, but found another type"
+  | None                => undefined "Error : no value at this address"
+  end.
+
+  Definition writePDflag (p : page) (idx : index) (flag : bool) : SAM unit :=
+  perform s := get in
+  let entry := lookup p idx (memory s) beqPage beqIndex in
+  match entry with
+  | Some (VE vir_entry) =>
+    let updated_entry := {| pd := flag; va := (va vir_entry) |} in
+    modify (fun s => {|
+      currentPartition := (currentPartition s);
+      memory := add p idx (VE updated_entry) (memory s) beqPage beqIndex
+    |})
+  | Some _ => undefined "Error : expected to find a virtual entry, but found another type"
+  | None   => undefined "Error : no value at this address"
+  end.
+
+  Definition readIndex (p : page) (idx : index) : SAM index :=
+  perform s := get in
+  let entry := lookup p idx (memory s) beqPage beqIndex in
+  match entry with
+  | Some (I i)  => ret i
+  | Some (VA _) => undefined "Error : expected to find an index, but found a virtual address"
+  | Some _      => undefined "Error : expected to find an index, but found another type"
+  | None        => undefined "Error : no value at this address"
+  end.
+
+  Definition writeIndex (p : page) (idx : index) (idx_to_write : index) : SAM unit :=
+  perform s := get in
+  modify (fun s => {|
+    currentPartition := (currentPartition s);
+    memory := add p idx (I idx_to_write) (memory s) beqPage beqIndex
+  |}).
+
+  Program Definition getMaxIndex : SAM index:=
+  if gt_dec tableSize 0
+  then
+    ret (Build_index_s (tableSize - 1) _)
+  else undefined "Error : tableSize is negative, can not build maxIndex".
+
+  Definition checkRights (r w e : bool) :=
+  if (r && w && e)
+  then
+    ret true
+  else ret (true || w).
+
+
+  Definition tableSizeLowerBound := 14.
+  Axiom tableSizeBigEnough : tableSize > tableSizeLowerBound.
+  Program Definition maxFreeLL : SAM index := 
+  ret (Build_index_s ((Coq.Init.Nat.div2 tableSize) - 2) _).
+  Next Obligation.
+  lia.
+  Qed.
+  Next Obligation.
+  assert(Init.Nat.div2 tableSize < tableSize).
+  apply Nat.lt_div2.
+  assert(tableSize > tableSizeLowerBound) by apply tableSizeBigEnough.
+  unfold tableSizeLowerBound in H.
+  lia.
+  lia.
+  Qed.
+
+  Definition defaultIndex := CIndex 0.
+
+  Definition getIndexOfAddr (va : vaddr) (l : level) : SAM index :=
+    ret ( nth ((length va) - (l + 2)) va defaultIndex ).
+
+  Program Definition getNbLevel : SAM level:=
+  if gt_dec nbLevel 0
+  then
+    ret (Build_level_s (nbLevel -1) _ )
+  else
+    undefined "Error : nbLevel is negative, can not return a neagative number".
+  Next Obligation.
+  lia.
+  Qed.
+
+  Definition prepareType (val1 : bool) (val2 : vaddr) : SAM boolvaddr :=
+  ret (Build_boolvaddr_s val1 val2).
+
+  Definition PDidx := CIndex 2.   (* page directory *)
+  Definition getPDidx : SAM index := ret PDidx.
+
+  Program Definition index_succ (n : index) : SAM index :=
+  let isucc := n+1 in
+  if (lt_dec isucc tableSize )
+  then
+    ret (Build_index_s isucc _ )
+  else  undefined "Error : provided index is bigger than the maximum expected index".
+
+  Definition getPd partition : SAM page :=
+  perform idxPD := getPDidx in
+  perform idx := index_succ idxPD in
+  readPhysical partition idx.
+
+  Definition defaultVAddr := CVaddr (repeat (CIndex 0) (nbLevel+1)).
+
+  Definition readVirtualUser (p : page) (idx : index) : SAM vaddr :=
+  perform s := get in
+  let entry :=  lookup p idx (memory s) beqPage beqIndex  in
+  match entry with
+  | Some (VA vaddr) => ret vaddr
+  | Some _      => ret defaultVAddr
+  | None        => ret defaultVAddr
+  end.
+
+  Definition level_eqb (a b : level) : SAM bool := ret (a =? b).
+  Definition fstLevel :=  CLevel 0.
+
+  Definition page_eqb (p1 : page) (p2 : page) : SAM bool := ret (p1 =? p2).
+
+  Definition comparePageToNull (p : page) : SAM bool :=
+  perform nullPaddr := ret defaultPage in
+  page_eqb nullPaddr p.
+
+  Program Definition level_pred (n : level) : SAM level :=
+  if gt_dec n 0
+  then
+  let ipred := n-1 in
+  ret (Build_level_s ipred _ )
+  else undefined "Error : level is less than zero, cannot get the preceding level".
+  Next Obligation.
+  destruct n; cbn; lia.
+  Qed.
+
+  (** The 'getTableAddrAux' returns the reference to the last page table  *)
+  Fixpoint translateAux timeout (pd : page) (va : vaddr) (l : level) :=
+  match timeout with
+  | 0          => ret defaultPage
+  | S timeout1 =>
+    perform isFstLevel := level_eqb l fstLevel in
+    if isFstLevel
+    then ret pd
+    else
+      perform idx := getIndexOfAddr va l in
+      perform addr := readPhyEntry pd idx in
+      perform isNull := comparePageToNull addr in
+      if isNull
+      then ret defaultPage
+      else
+        perform p := level_pred l in
+        translateAux timeout1 addr va p
+  end.
+
+  (** The 'translate' *)
+  Definition  translate (pd : page) (va : vaddr) (l : level) : SAM (option page)  :=
+  perform lastTable := translateAux nbLevel pd va l in 
+  perform isNull := comparePageToNull lastTable in
+  if isNull then ret None else
+  perform idx :=  getIndexOfAddr va fstLevel in
+  perform ispresent := readPresent lastTable idx in 
+  perform isaccessible := readAccessible lastTable idx in
+  if (ispresent && isaccessible) then  
+  perform phypage := readPhyEntry lastTable idx in 
+  ret (Some phypage)
+  else ret None.
+
+
+  Definition fetchVirtual (va : vaddr) (idx : index) : SAM vaddr :=
+  perform currentPartition := getCurPartition in
+  perform currentPD := getPd currentPartition in
+  perform nbL := getNbLevel in
+  perform optionphyPage := translate currentPD va nbL in
+  match optionphyPage with 
+  | None         => ret defaultVAddr
+  | Some phyPage => readVirtualUser phyPage idx
+  end.
+
+  Definition storeVirtual (va : vaddr) (idx : index) (vaToStore : vaddr) : SAM unit:=
+  perform currentPartition := getCurPartition in
+  perform currentPD := getPd currentPartition in
+  perform nbL := getNbLevel in
+  perform optionphyPage := translate currentPD va nbL in
+  match optionphyPage with
+  | None => ret tt
+  | Some phyPage => writeVirtual phyPage idx vaToStore
+  end.
+
+  Definition setInterruptMask (mask : interruptMask) : SAM unit :=
+  ret tt.
+
+  Definition getInterruptMaskFromCtx (context : contextAddr) : SAM interruptMask :=
+  ret int_mask_d.
+
+  Definition noInterruptRequest (flags : interruptMask) : SAM bool :=
+  ret true.
+
+  Definition updateMMURoot(pageDir : page) : SAM unit :=
+  ret tt.
+
+  Definition multiplexer := CPage 1.
+  Definition getMultiplexer : SAM page :=
+  ret multiplexer.
+
+  Definition loadContext (contextToLoad : contextAddr) (enforce_interrupt : bool) : SAM unit :=
+  ret tt.
+
+End IsolationStateMonad.
