src/model/Meta/InterfaceModel.v
@@ -1,0 +1,47 @@
+From Pip.Model.Meta Require Import TypesModel StateModel StateAgnosticMonad.
+
+Module Type InterfaceModel (Export Types : TypesModel)
+                           (Export State : StateModel).
+
+  Module SAMM := StateAgnosticMonad State.
+  Export SAMM.
+  (* Monad Interface *)
+
+  Parameter getCurPartition : SAM page.
+  Parameter updateCurPartition : page -> SAM unit.
+  Parameter readVirtual : page -> index -> SAM vaddr.
+  Parameter readPhysical : page -> index -> SAM page.
+  Parameter readVirEntry : page -> index -> SAM vaddr.
+  Parameter readPhyEntry : page -> index -> SAM page.
+  Parameter writeVirtual : page -> index -> vaddr -> SAM unit.
+  Parameter writePhysical : page -> index -> page -> SAM unit.
+  Parameter writeVirEntry : page -> index -> vaddr -> SAM unit.
+  Parameter writePhyEntry : page -> index -> page -> bool -> bool -> bool -> bool -> bool -> SAM unit.
+  Parameter mapKernel : page -> index -> SAM unit.
+  Parameter readAccessible : page -> index -> SAM bool.
+  Parameter writeAccessible : page -> index -> bool -> SAM unit.
+  Parameter readPresent : page -> index -> SAM bool.
+  Parameter writePresent : page -> index -> bool -> SAM unit.
+  Parameter readPDflag : page -> index -> SAM bool.
+  Parameter writePDflag : page -> index -> bool -> SAM unit.
+  Parameter readIndex : page -> index -> SAM index.
+  Parameter writeIndex : page -> index -> index -> SAM unit.
+  Parameter getMaxIndex : SAM index.
+  Parameter checkRights : bool -> bool -> bool -> SAM bool.
+  Parameter maxFreeLL : SAM index.
+  Parameter getIndexOfAddr : vaddr -> level -> SAM index.
+  Parameter getNbLevel : SAM level.
+  Parameter prepareType : bool -> vaddr -> SAM boolvaddr.
+  Parameter getPd : page -> SAM page.
+  Parameter readVirtualUser : page -> index -> SAM vaddr.
+  Parameter fetchVirtual : vaddr -> index -> SAM vaddr.
+  Parameter storeVirtual : vaddr -> index -> vaddr -> SAM unit.
+  Parameter setInterruptMask : interruptMask -> SAM unit.
+  Parameter getInterruptMaskFromCtx : contextAddr -> SAM interruptMask.
+  Parameter noInterruptRequest : interruptMask -> SAM bool.
+  Parameter updateMMURoot : page -> SAM unit.
+  Parameter getMultiplexer : SAM page.
+  Parameter page_eqb : page -> page -> SAM bool.
+  Parameter loadContext : contextAddr -> bool -> SAM unit.
+
+End InterfaceModel.
