src/model/Meta/TypesModel.v
@@ -1,0 +1,31 @@
+Module Type TypesModel.
+
+  Parameter index : Type.
+  Parameter index_d : index.
+  Parameter page  : Type.
+  Parameter page_d : page.
+  Parameter paddr : Type.
+  Parameter vaddr : Type.
+  Parameter level : Type.
+  Parameter level_d : level.
+  Parameter count : Type.
+  Parameter count_d : count.
+  Parameter boolvaddr : Type.
+  Parameter userValue : Type.
+  Parameter contextAddr : Type.
+  Parameter interruptMask : Type.
+  Parameter int_mask_d : interruptMask.
+
+  Inductive yield_checks : Type :=
+| FAIL_INVALID_INT_LEVEL
+| FAIL_INVALID_CTX_SAVE_INDEX
+| FAIL_CALLER_CONTEXT_SAVE
+| FAIL_UNAVAILABLE_TARGET_VIDT
+| FAIL_UNAVAILABLE_TARGET_CTX
+| FAIL_UNAVAILABLE_CALLER_VIDT
+| FAIL_ROOT_CALLER
+| FAIL_INVALID_CHILD
+| FAIL_MASKED_INTERRUPT
+| SUCCESS.
+
+End TypesModel.
