src/model/Meta/StateModel.v
@@ -1,0 +1,5 @@
+Module Type StateModel.
+
+  Parameter state : Type.
+
+End StateModel.
