src/model/StateParameter.v
@@ -1,5 +1,0 @@
-Module Type StateParameter.
-
-  Parameter state : Type.
-
-End StateParameter.
